README.md
@@ -8,7 +8,7 @@ First, there are some proven correct [deciders](https://wiki.bbchallenge.org/wik
 
 Then, for the rest of the TMs, we can write individual proof for them. If a TM (up to equivalence) haven't been proven, it becomes a holdout.
 
-For BB(6), there're about 1800 holdouts, while about 250 individual proofs haven't been translated to Rocq.
+For BB(6), there're about 1700 holdouts, while about 250 individual proofs haven't been translated to Rocq.
 
 For BB(2,5), there're about 70 holdouts, while about 10 individual proofs haven't been translated to Rocq.
 
